theories/utils/contribution.v
@@ -20,7 +20,7 @@ From iris.proofmode Require Export tactics.
 From iris.algebra Require Import excl auth csum gmultiset numbers.
 From iris.algebra Require Export local_updates.
 
-Class contributionG Σ (A : ucmraT) `{!CmraDiscrete A} := {
+Class contributionG Σ (A : ucmra) `{!CmraDiscrete A} := {
   contribution_inG :> inG Σ
     (authR (optionUR (csumR (prodR positiveR A) (exclR unitO))))
 }.
